PrimitiveRecognizers.v
@@ -17,3 +17,15 @@ Definition is_lambda (v: tree): tree :=
   | notype_lambda _ => ttrue
   | _ => tfalse
   end.
+
+Definition is_unary_primitive (v: tree): tree :=
+  match v with
+  | unary_primitive _ _ => ttrue
+  | _ => tfalse
+  end.
+
+Definition is_binary_primitive (v: tree): tree :=
+  match v with
+  | binary_primitive _ _ _ => ttrue
+  | _ => tfalse
+  end.
