SmallStep.v
@@ -4,6 +4,7 @@ Require Import Relations.
 Require Export SystemFR.PrimitiveSize.
 Require Export SystemFR.PrimitiveRecognizers.
 
+
 Inductive cbv_value: tree -> Prop :=
 | IVUnit: cbv_value uu
 | IVZero: cbv_value zero
@@ -59,12 +60,14 @@ Proof.
   - exists (S n); steps.
 Qed.
 
+
 Ltac is_nat_value_buildable :=
   match goal with
   | H: is_nat_value ?v |- _ =>
     poseNew (Mark v "is_nat_value_buildable");
     pose proof (is_nat_value_buildable v H)
   end.
+
 
 Lemma tree_size_build_nat:
   forall n, tree_size (build_nat n) = n.
@@ -101,6 +104,7 @@ Lemma cbv_value_is_lambda:
 Proof.
   destruct v; steps.
 Qed.
+
 
 Hint Immediate is_nat_value_build_nat: values.
 Hint Immediate cbv_value_build_nat: values.
@@ -196,6 +200,58 @@ Inductive scbv_step: tree -> tree -> Prop :=
       ~ top_level_var v ->
       boolean_recognizer 2 v ~> is_lambda v
 
+(* Primitive beta reduction *)
+| SPBetaPlus: forall v1 v2 n1 n2,
+    v1 = build_nat n1 ->
+    v2 = build_nat n2 ->
+    scbv_step (binary_primitive plus v1 v2) (build_nat (n1 + n2))
+| SPBetaMinus: forall v1 v2 n1 n2,
+    v1 = build_nat n1 ->
+    v2 = build_nat n2 ->
+    scbv_step (binary_primitive minus v1 v2) (build_nat (n1 - n2))
+| SPBetaMul: forall v1 v2 n1 n2,
+    v1 = build_nat n1 ->
+    v2 = build_nat n2 ->
+    scbv_step (binary_primitive mul v1 v2) (build_nat (n1 * n2))
+| SPBetaDiv: forall v1 v2 n1 n2,
+    v1 = build_nat n1 ->
+    v2 = build_nat (S n2) ->
+    scbv_step (binary_primitive div v1 v2) (build_nat (PeanoNat.Nat.div n1 (S n2)))
+| SPBetaEq: forall v1 v2 n1 n2,
+    v1 = build_nat n1 ->
+    v2 = build_nat n2 ->
+    scbv_step (binary_primitive eq  v1 v2) (if PeanoNat.Nat.eqb n1 n2 then ttrue else tfalse)
+| SPBetaNeq: forall v1 v2 n1 n2,
+    v1 = build_nat n1 ->
+    v2 = build_nat n2 ->
+    scbv_step (binary_primitive neq v1 v2) (if (PeanoNat.Nat.eq_dec n1 n2) then tfalse else ttrue)
+| SPBetaLt: forall v1 v2 n1 n2,
+    v1 = build_nat n1 ->
+    v2 = build_nat n2 ->
+    scbv_step (binary_primitive lt  v1 v2) (if PeanoNat.Nat.ltb n1 n2 then ttrue else tfalse)
+| SPBetaLeq: forall v1 v2 n1 n2,
+    v1 = build_nat n1 ->
+    v2 = build_nat n2 ->
+    scbv_step (binary_primitive leq v1 v2) (if PeanoNat.Nat.leb n1 n2 then ttrue else tfalse)
+| SPBetaGt: forall v1 v2 n1 n2,
+    v1 = build_nat n1 ->
+    v2 = build_nat n2 ->
+    scbv_step (binary_primitive gt  v1 v2) (if PeanoNat.Nat.leb n1 n2 then tfalse else ttrue)
+| SPBetaGeq: forall v1 v2 n1 n2,
+    v1 = build_nat n1 ->
+    v2 = build_nat n2 ->
+    scbv_step (binary_primitive geq v1 v2) (if PeanoNat.Nat.ltb n1 n2 then tfalse else ttrue)
+
+| SPBetaNot1: scbv_step (unary_primitive Not ttrue) tfalse
+| SPBetaNot2: scbv_step (unary_primitive Not tfalse) ttrue
+
+| SPBetaAnd1: scbv_step (binary_primitive And ttrue ttrue) ttrue
+| SPBetaAnd2: scbv_step (binary_primitive And ttrue tfalse) tfalse
+
+| SPBetaOr1: scbv_step (binary_primitive Or tfalse tfalse) tfalse
+| SPBetaOr2: scbv_step (binary_primitive Or tfalse ttrue) ttrue
+
+
 (* reduction inside terms *)
 | SPAppLeft: forall t1 t2 t,
     t1 ~> t2 ->
@@ -224,6 +280,17 @@ Inductive scbv_step: tree -> tree -> Prop :=
 | SPMatch: forall t1 t2 t0 ts,
     t1 ~> t2 ->
     tmatch t1 t0 ts ~> tmatch t2 t0 ts
+
+| SPUnaryPrimitive: forall o t1 t2,
+    scbv_step t1 t2 ->
+    scbv_step (unary_primitive o t1) (unary_primitive o t2)
+| SPBinaryPrimitive1: forall o t1 t2 t,
+    scbv_step t1 t2 ->
+    scbv_step (binary_primitive o t1 t) (binary_primitive o t2 t)
+| SPBinaryPrimitive2: forall o v t1 t2,
+    scbv_step t1 t2 ->
+    cbv_value v ->
+    scbv_step (binary_primitive o v t1) (binary_primitive o v t2)
 
 | SPIte: forall t1 t1' t2 t3,
     t1 ~> t1' ->
@@ -275,6 +342,8 @@ Ltac t_invert_step :=
   | H: pi2 _ ~> _ |- _ => inversion H; clear H
   | H: sum_match _ _ _ ~> _ |- _ => inversion H; clear H
   | H: tsize _ ~> _ |- _ => inversion H; clear H
+  | H: unary_primitive _ _ ~> _ |- _ => inversion H; clear H
+  | H: binary_primitive _ _ _ ~> _ |- _ => inversion H; clear H
   end.
 
 Lemma evaluate_step:
@@ -329,6 +398,14 @@ Qed.
 
 Hint Immediate is_nat_value_value: values.
 
+Lemma evaluate_step_build_nat:
+  forall t n,
+    scbv_step (build_nat n) t -> False.
+Proof.
+  eauto using evaluate_step2 with values.
+Qed.
+Hint Immediate evaluate_step_build_nat: smallstep.
+
 Lemma is_nat_value_erased:
   forall v,
     is_nat_value v ->
@@ -342,6 +419,7 @@ Hint Immediate is_nat_value_erased: erased.
 Ltac no_step :=
   match goal with
   | H: cbv_value err |- _ => inversion H
+  | H: build_nat ?n ~> ?t |- _ => apply evaluate_step_build_nat in H; apply False_ind, H
   | H1: cbv_value ?v,
     H2: ?v ~> ?t |- _ =>
     apply False_ind; apply evaluate_step with v t; auto 2
@@ -369,7 +447,7 @@ Lemma deterministic_step:
       t2 = t3.
 Proof.
   induction 1; repeat step || t_equality;
-    try solve [ repeat step || t_invert_step || no_step || t_equality ].
+    try solve [ repeat step || t_invert_step || no_step || t_equality || build_nat_inj ].
 Qed.
 
 Ltac deterministic_step :=
